theories/algebra/algebra.v
@@ -1,1 +1,0 @@
-From HypVeri.algebra Require Export algebra_base mem reg mailbox pagetable trans.
