theories/algebra/mem.v
@@ -1,5 +1,5 @@
 From HypVeri.algebra Require Import base.
-From HypVeri Require Import lang_misc.
+From HypVeri Require Import lang_extra.
 
 Section mem_rules.
   Context `{vmG : !gen_VMG Σ}.
