theories/lang/current_extra.v
@@ -1,0 +1,56 @@
+From HypVeri Require Import machine machine_extra.
+From HypVeri.algebra Require Import base.
+
+Lemma update_current_vmid_preserve_reg σ i :
+  get_reg_gmap (update_current_vmid σ i) = get_reg_gmap σ.
+Proof. f_equal. Qed.
+
+Lemma update_current_vmid_preserve_mem σ i :
+  get_mem (update_current_vmid σ i) = get_mem σ.
+Proof. f_equal. Qed.
+
+
+Lemma update_current_vmid_preserve_tx σ i :
+  get_tx_agree (update_current_vmid σ i) = (get_tx_agree σ).
+Proof. f_equal. Qed.
+
+Lemma update_current_vmid_preserve_rx1 σ i :
+  get_rx_agree (update_current_vmid σ i) = (get_rx_agree σ).
+Proof. f_equal. Qed.
+
+
+Lemma update_current_vmid_preserve_rx2 σ i :
+  get_rx_gmap (update_current_vmid σ i) = (get_rx_gmap σ).
+Proof. f_equal. Qed.
+
+Lemma update_current_vmid_preserve_pt σ i i':
+  get_vm_page_table (update_current_vmid σ i) i' = get_vm_page_table σ i'.
+Proof. f_equal. Qed.
+
+Lemma update_current_vmid_preserve_owned σ i :
+  get_owned_gmap (update_current_vmid σ i) = (get_owned_gmap σ).
+Proof. f_equal. Qed.
+
+Lemma update_current_vmid_preserve_access σ i :
+  get_access_gmap (update_current_vmid σ i) = (get_access_gmap σ).
+Proof. f_equal. Qed.
+
+Lemma update_current_vmid_preserve_excl σ i :
+  get_excl_gmap (update_current_vmid σ i) = (get_excl_gmap σ).
+Proof. f_equal. Qed.
+
+Lemma update_current_vmid_preserve_trans σ i :
+  get_trans_gmap (update_current_vmid σ i) = (get_trans_gmap σ).
+Proof. f_equal. Qed.
+
+Lemma update_current_vmid_preserve_trans' σ i :
+  get_transactions (update_current_vmid σ i) = (get_transactions σ).
+Proof. f_equal. Qed.
+
+Lemma update_current_vmid_preserve_hpool σ i :
+  get_hpool_gset (update_current_vmid σ i) = (get_hpool_gset σ).
+Proof. f_equal. Qed.
+
+Lemma update_current_vmid_preserve_retri σ i :
+  get_retri_gmap (update_current_vmid σ i) = (get_retri_gmap σ).
+Proof. f_equal. Qed.
