theories/lang/reg_extra.v
@@ -1,0 +1,352 @@
+From HypVeri Require Import machine.
+From HypVeri.algebra Require Import base.
+
+
+Lemma update_reg_global_preserve_current_vm σ i r w :
+  (get_current_vm (update_reg_global σ i r w)) = (get_current_vm σ).
+Proof. f_equal. Qed.
+
+Lemma update_reg_global_preserve_mem σ i r w : get_mem (update_reg_global σ i r w) = get_mem σ.
+Proof. f_equal. Qed.
+
+Lemma update_reg_global_preserve_tx σ i r w :
+  get_tx_agree (update_reg_global σ i r w) = (get_tx_agree σ).
+Proof. f_equal. Qed.
+
+Lemma update_reg_global_preserve_rx1 σ i r w :
+  get_rx_agree (update_reg_global σ i r w) = (get_rx_agree σ).
+Proof. f_equal. Qed.
+
+Lemma update_reg_global_preserve_rx2 σ i r w :
+  get_rx_gmap (update_reg_global σ i r w) = (get_rx_gmap σ).
+Proof. f_equal. Qed.
+
+Lemma update_reg_global_preserve_pt σ i i' r w:
+  get_vm_page_table (update_reg_global σ i r w) i' = get_vm_page_table σ i'.
+Proof. f_equal. Qed.
+
+Lemma update_reg_global_preserve_owned σ i r w :
+  get_owned_gmap (update_reg_global σ i r w) = (get_owned_gmap σ).
+Proof. f_equal. Qed.
+
+Lemma update_reg_global_preserve_access σ i r w :
+  get_access_gmap (update_reg_global σ i r w) = (get_access_gmap σ).
+Proof. f_equal. Qed.
+
+Lemma update_reg_global_preserve_excl σ i r w :
+  get_excl_gmap (update_reg_global σ i r w) = (get_excl_gmap σ).
+Proof. f_equal. Qed.
+
+Lemma update_reg_global_preserve_trans σ i r w :
+  get_trans_gmap (update_reg_global σ i r w) = (get_trans_gmap σ).
+Proof. f_equal. Qed.
+
+Lemma update_reg_global_preserve_trans' σ i r w :
+  get_transactions (update_reg_global σ i r w) = (get_transactions σ).
+Proof. f_equal. Qed.
+
+Lemma update_reg_global_preserve_hpool σ i r w :
+  get_hpool_gset (update_reg_global σ i r w) = (get_hpool_gset σ).
+Proof. f_equal. Qed.
+
+Lemma update_reg_global_preserve_retri σ i r w :
+  get_retri_gmap (update_reg_global σ i r w) = (get_retri_gmap σ).
+Proof. f_equal. Qed.
+
+Lemma update_offset_PC_preserve_current_vm σ o :
+  (get_current_vm (update_offset_PC σ o )) = (get_current_vm σ).
+Proof.
+  rewrite /update_offset_PC /get_current_vm.
+  destruct (get_vm_reg_file σ σ.1.1.2 !! PC);eauto.
+Qed.
+
+Lemma update_offset_PC_preserve_mem σ o :
+  get_mem (update_offset_PC σ o) = get_mem σ.
+Proof.
+  unfold update_offset_PC.
+  destruct (get_vm_reg_file σ (get_current_vm σ) !! PC).
+  f_equal.
+  done.
+Qed.
+
+Lemma update_offset_PC_preserve_tx σ o :
+  get_tx_agree (update_offset_PC σ o) = get_tx_agree σ.
+Proof.
+  unfold update_offset_PC.
+  destruct (get_vm_reg_file σ (get_current_vm σ) !! PC).
+  rewrite /update_reg update_reg_global_preserve_tx;done.
+  done.
+Qed.
+
+Lemma update_offset_PC_preserve_rx1 σ o :
+  get_rx_agree (update_offset_PC σ o) = get_rx_agree σ.
+Proof.
+  unfold update_offset_PC.
+  destruct (get_vm_reg_file σ (get_current_vm σ) !! PC).
+  rewrite /update_reg update_reg_global_preserve_rx1;done.
+  done.
+Qed.
+
+Lemma update_offset_PC_preserve_rx2 σ o :
+  get_rx_gmap (update_offset_PC σ o) = get_rx_gmap σ.
+Proof.
+  unfold update_offset_PC.
+  destruct (get_vm_reg_file σ (get_current_vm σ) !! PC).
+  rewrite /update_reg update_reg_global_preserve_rx2;done.
+  done.
+Qed.
+
+Lemma update_offset_PC_preserve_owned σ o :
+  get_owned_gmap (update_offset_PC σ o) = get_owned_gmap σ.
+Proof.
+  unfold update_offset_PC.
+  destruct (get_vm_reg_file σ (get_current_vm σ) !! PC).
+  rewrite /update_reg update_reg_global_preserve_owned;done.
+  done.
+Qed.
+
+Lemma update_offset_PC_preserve_access σ o :
+  get_access_gmap (update_offset_PC σ o) = get_access_gmap σ.
+Proof.
+  unfold update_offset_PC.
+  destruct (get_vm_reg_file σ (get_current_vm σ) !! PC).
+  rewrite /update_reg update_reg_global_preserve_access;done.
+  done.
+Qed.
+
+Lemma update_offset_PC_preserve_check_access σ o a:
+  check_access_addr (update_offset_PC σ o) (get_current_vm σ) a
+  = check_access_addr  σ (get_current_vm σ) a.
+Proof.
+  rewrite /update_offset_PC /check_access_addr /check_access_page.
+  simpl.
+  destruct (get_vm_reg_file σ (get_current_vm σ) !! PC);eauto.
+Qed.
+
+Lemma update_offset_PC_preserve_excl σ o :
+  get_excl_gmap (update_offset_PC σ o) = get_excl_gmap σ.
+Proof.
+  unfold update_offset_PC.
+  destruct (get_vm_reg_file σ (get_current_vm σ) !! PC).
+  rewrite /update_reg update_reg_global_preserve_excl;done.
+  done.
+Qed.
+
+Lemma update_offset_PC_preserve_trans σ o :
+  get_trans_gmap (update_offset_PC σ o) = get_trans_gmap σ.
+Proof.
+  unfold update_offset_PC.
+  destruct (get_vm_reg_file σ (get_current_vm σ) !! PC).
+  rewrite /update_reg update_reg_global_preserve_trans;done.
+  done.
+Qed.
+
+Lemma update_offset_PC_preserve_trans' σ o :
+  get_transactions (update_offset_PC σ o) = get_transactions σ.
+Proof.
+  unfold update_offset_PC.
+  destruct (get_vm_reg_file σ (get_current_vm σ) !! PC).
+  rewrite /update_reg update_reg_global_preserve_trans';done.
+  done.
+Qed.
+
+Lemma update_offset_PC_preserve_hpool σ o :
+  get_hpool_gset (update_offset_PC σ o) = get_hpool_gset σ.
+Proof.
+  unfold update_offset_PC.
+  destruct (get_vm_reg_file σ (get_current_vm σ) !! PC).
+  rewrite /update_reg update_reg_global_preserve_hpool;done.
+  done.
+Qed.
+
+Lemma update_offset_PC_preserve_retri σ o :
+  get_retri_gmap (update_offset_PC σ o) = get_retri_gmap σ.
+Proof.
+  unfold update_offset_PC.
+  destruct (get_vm_reg_file σ (get_current_vm σ) !! PC).
+  rewrite /update_reg update_reg_global_preserve_retri;done.
+  done.
+Qed.
+
+Lemma get_reg_global_update_reg_global_ne_vmid {σ i j R1 R2 A B} :
+  i ≠ j ->
+  get_reg_global σ j R2 = Some B ->
+  get_reg_global (update_reg_global σ i R1 A) j R2 = Some B.
+Proof.
+  intros Hne Hlk.
+  rewrite /get_reg_global /get_vm_reg_file /get_reg_files /update_reg_global.
+  simpl.
+  rewrite vlookup_insert_ne; auto.
+Qed.
+
+Lemma get_reg_gmap_lookup_Some σ i r w :
+  (get_reg_gmap σ) !! (r,i)= Some w <->  get_vm_reg_file σ i !! r = Some w.
+Proof.
+  split.
+  - unfold get_reg_gmap.
+    intro HSome.
+    apply elem_of_list_to_map_2 in HSome.
+    apply elem_of_list_In in HSome.
+    apply in_flat_map in HSome.
+    destruct HSome  as [i'] .
+    destruct H as [HiIn].
+    apply in_map_iff in H.
+    destruct H as [p].
+    destruct H as [Heqn].
+    inversion Heqn ;subst;clear Heqn.
+    apply elem_of_list_In in H.
+      by apply elem_of_map_to_list' in H.
+  - intro HSome.
+    apply  elem_of_list_to_map_1'.
+    + intros.
+      apply elem_of_list_In in H.
+      apply in_flat_map in H.
+      destruct H as [i'].
+      destruct H as [Hi'In H].
+      apply in_map_iff in H.
+      destruct H as [p].
+      destruct H as [Heqn H].
+      apply elem_of_list_In in H.
+      apply elem_of_map_to_list' in H.
+      inversion Heqn;subst;clear Heqn.
+      rewrite H in HSome.
+        by inversion HSome.
+    + apply elem_of_list_In.
+      apply in_flat_map.
+      exists i.
+      split;[apply in_list_of_vmids|].
+      apply in_map_iff.
+      exists (r,w).
+      split;[done|].
+      apply elem_of_list_In.
+      apply elem_of_map_to_list'.
+      done.
+Qed.
+
+Lemma get_reg_gmap_lookup_None σ i r :
+  (get_reg_gmap σ) !! (r,i)= None <->  get_vm_reg_file σ i !! r = None.
+Proof.
+  split.
+  - destruct (get_vm_reg_file σ i !! r) as [w|]  eqn:Heqn;[|done].
+    intro HNone.
+    apply not_elem_of_list_to_map_2 in HNone.
+    exfalso.
+    apply HNone.
+    apply elem_of_list_In.
+    apply in_map_iff.
+    exists (r,i,w).
+    split;[done|].
+    apply in_flat_map.
+    exists i.
+    split;[apply in_list_of_vmids|].
+    apply in_map_iff.
+    exists (r,w).
+    split;[done|].
+    apply elem_of_list_In.
+    apply elem_of_map_to_list'.
+    by simplify_eq /=.
+  - intro HNone.
+    apply  not_elem_of_list_to_map_1.
+    intro.
+    apply elem_of_list_In in H.
+    apply in_map_iff in H.
+    destruct H as [p].
+    destruct H as [Heqn H].
+    apply elem_of_list_In in H.
+    apply elem_of_list_In in H.
+    apply in_flat_map in H.
+    inversion Heqn;subst;clear Heqn.
+    destruct H as [i'].
+    destruct H as [HIn H].
+    apply in_map_iff in H.
+    destruct H as [p2].
+    destruct H as [Heqn H].
+    apply elem_of_list_In in H.
+    apply elem_of_map_to_list' in H.
+    inversion Heqn;subst;clear H0.
+    inversion H1;subst;clear H1.
+    rewrite H in HNone.
+    by inversion HNone.
+Qed.
+
+Lemma get_reg_gmap_get_vm_reg_file σ (r:reg_name) (i:VMID) :
+  (get_reg_gmap σ) !! (r,i) = (get_vm_reg_file σ i) !! r.
+Proof.
+  destruct (get_reg_gmap σ !! (r, i)) eqn:Heqn.
+  apply get_reg_gmap_lookup_Some in Heqn;done.
+  apply get_reg_gmap_lookup_None in Heqn;done.
+Qed.
+
+Lemma get_reg_gmap_get_reg_Some σ (r:reg_name) (w:Word) (i:VMID) :
+  i= (get_current_vm σ)->
+  (get_reg_gmap σ) !! (r,i) = Some w <-> ((get_reg σ r) = Some w).
+Proof.
+  intros.
+  rewrite get_reg_gmap_get_vm_reg_file.
+  unfold get_reg,get_reg_global;subst;done.
+Qed.
+
+Lemma update_reg_global_update_reg σ i r w :
+  is_Some((get_reg_gmap σ) !! (r,i)) ->
+  get_reg_gmap (update_reg_global σ i r w) = <[(r,i) := w]>(get_reg_gmap σ).
+Proof.
+  intros.
+  rewrite  /update_reg_global.
+  apply map_eq.
+  intro j.
+  destruct( decide (j=(r,i)) ).
+  - subst j.
+    rewrite lookup_insert.
+    rewrite get_reg_gmap_get_vm_reg_file.
+    rewrite /get_vm_reg_file /get_reg_files.
+    simpl.
+    rewrite -> (vlookup_insert i _  _).
+      by rewrite lookup_insert.
+  - destruct ((get_reg_gmap σ) !! j) eqn:Heqn;
+      rewrite lookup_insert_ne;[|done | |done];
+        rewrite -> Heqn;
+        destruct j as [r' i'];
+        rewrite ->get_reg_gmap_get_vm_reg_file in Heqn;
+        rewrite ->get_reg_gmap_get_vm_reg_file;
+        destruct (decide (i=i'));
+        destruct (decide (r=r'));
+        subst;
+        try contradiction;
+        rewrite - Heqn;
+        rewrite /get_vm_reg_file /get_reg_files;simpl.
+    + rewrite -> (vlookup_insert i' _ _).
+        by rewrite lookup_insert_ne ;[|done].
+    + by rewrite vlookup_insert_ne.
+    + by rewrite vlookup_insert_ne.
+    + rewrite -> (vlookup_insert i' _ _).
+        by rewrite lookup_insert_ne ;[|done].
+    + by rewrite vlookup_insert_ne ;[|done].
+    + by rewrite vlookup_insert_ne ;[|done].
+Qed.
+
+Lemma update_offset_PC_update_PC1 σ i (w:Word) (o:Z):
+  i=get_current_vm σ -> ((get_reg_gmap σ) !! (PC,i) = Some w) ->
+  get_reg_gmap (update_offset_PC σ o) = <[(PC,i) := (w ^+ o)%f]>(get_reg_gmap σ).
+Proof.
+  intros.
+  rewrite /update_offset_PC.
+  remember H0.
+  clear Heqe.
+  rewrite /get_reg_gmap /update_reg_global in H0.
+  apply elem_of_list_to_map_2 in H0.
+  apply elem_of_list_In in H0.
+  apply in_flat_map in H0.
+  destruct H0.
+  destruct H0.
+  apply in_map_iff in H1.
+  destruct H1.
+  destruct H1.
+  inversion H1;subst;clear H1.
+  apply elem_of_list_In in H2.
+  apply elem_of_map_to_list' in H2.
+  rewrite H2.
+  rewrite /update_reg.
+  apply update_reg_global_update_reg.
+  exists x0.2.
+    by rewrite H4.
+Qed.
