theories/lang/trans_extra.v
@@ -1,0 +1,434 @@
+From HypVeri Require Import machine machine_extra tactics.
+From HypVeri.algebra Require Import base.
+
+Lemma insert_transaction_preserve_current_vm σ h trans:
+  get_current_vm (insert_transaction σ h trans) = get_current_vm σ.
+Proof. f_equal. Qed.
+
+Lemma insert_transaction_preserve_regs σ h trans:
+  get_reg_gmap (insert_transaction σ h trans) = get_reg_gmap σ.
+Proof. f_equal. Qed.
+
+Lemma insert_transaction_preserve_mem σ h trans:
+  get_mem (insert_transaction σ h trans) = get_mem σ.
+Proof. f_equal. Qed.
+
+Lemma insert_transaction_preserve_tx σ h trans:
+  get_tx_agree (insert_transaction σ h trans) = get_tx_agree σ.
+Proof. f_equal. Qed.
+
+Lemma insert_transaction_preserve_rx1 σ h trans:
+  get_rx_agree (insert_transaction σ h trans) = get_rx_agree σ.
+Proof. f_equal. Qed.
+
+Lemma insert_transaction_preserve_rx2 σ h trans:
+  get_rx_gmap(insert_transaction σ h trans) = get_rx_gmap σ.
+Proof. f_equal. Qed.
+
+Lemma insert_transaction_preserve_rx  σ h trans:
+  (get_rx_agree (insert_transaction σ h trans), get_rx_gmap (insert_transaction σ h trans) ) =
+  (get_rx_agree σ, get_rx_gmap σ).
+Proof. by rewrite insert_transaction_preserve_rx1 insert_transaction_preserve_rx2 . Qed.
+
+Lemma insert_transaction_preserve_owned σ h trans:
+  get_owned_gmap (insert_transaction σ h trans) = get_owned_gmap σ.
+Proof. f_equal. Qed.
+Lemma insert_transaction_preserve_access σ h trans:
+  get_access_gmap (insert_transaction σ h trans) = get_access_gmap σ.
+Proof. f_equal. Qed.
+
+Lemma insert_transaction_preserve_excl σ h trans:
+  get_excl_gmap (insert_transaction σ h trans) = get_excl_gmap σ.
+Proof. f_equal. Qed.
+
+Lemma insert_transaction_update_transactions{Info:Type}{σ} (proj: transaction -> Info) h tran:
+  (get_transactions_gmap (insert_transaction σ h tran) proj)
+  = <[h:= (proj tran)]>(get_transactions_gmap σ proj).
+Proof.
+  rewrite /get_transactions_gmap //=.
+  apply map_eq.
+  intro.
+  destruct (decide (h=i)).
+  - subst i;rewrite lookup_insert.
+    apply elem_of_list_to_map_1'.
+    + intros.
+      inv_map_in.
+      inversion H.
+      subst h.
+      destruct x;simpl.
+      apply elem_of_list_In in H0.
+      apply elem_of_map_to_list' in H0.
+      simpl in H0.
+      rewrite lookup_insert in H0.
+      inversion H0;subst t.
+      done.
+    + inv_map_in.
+      exists (h, tran).
+      split.
+      done.
+      apply elem_of_list_In.
+      apply elem_of_map_to_list'.
+      apply lookup_insert.
+  - rewrite lookup_insert_ne;eauto.
+    destruct (list_to_map (map (λ p : Addr * transaction, (p.1, (proj p.2) )) (map_to_list (get_transactions σ).1)) !! i) eqn:Heqn.
+    + apply elem_of_list_to_map_2 in Heqn.
+      apply elem_of_list_In in Heqn.
+      apply in_map_iff in Heqn.
+      destruct Heqn.
+      destruct H.
+      inversion H.
+      subst i.
+      destruct x;simpl in *.
+      apply elem_of_list_In in H0.
+      apply elem_of_map_to_list' in H0.
+      simpl in H0.
+      apply elem_of_list_to_map_1'.
+      * intros.
+        inv_map_in.
+        inversion H1.
+        subst f.
+        destruct x;simpl in *.
+        apply elem_of_list_In in H2.
+        apply elem_of_map_to_list' in H2.
+        simpl in H2.
+        rewrite lookup_insert_ne in H2;eauto.
+        rewrite H2 in H0.
+        inversion H0;subst t.
+        done.
+      * inv_map_in.
+        exists (f, t).
+        split.
+        done.
+        apply elem_of_list_In.
+        apply elem_of_map_to_list'.
+        simpl.
+        rewrite lookup_insert_ne;eauto.
+    + apply not_elem_of_list_to_map_1.
+      apply not_elem_of_list_to_map_2 in Heqn.
+      intro.
+      apply Heqn.
+      apply elem_of_list_In in H.
+      apply in_map_iff in H.
+      destruct H.
+      destruct H.
+      destruct H.
+      apply elem_of_list_In in H0.
+      apply elem_of_list_In in H0.
+      apply in_map_iff in H0.
+      destruct H0.
+      destruct H.
+      destruct x;inversion H.
+      apply elem_of_list_In in H0.
+      apply elem_of_map_to_list' in H0.
+      simpl in *.
+      subst f.
+      rewrite lookup_insert_ne in H0;eauto.
+      apply elem_of_list_In.
+      apply in_map_iff.
+      exists (x0.1,i).
+      split;[done|].
+      apply in_map_iff.
+      exists (x0.1,x0.2).
+      subst i;split;[done|].
+      apply elem_of_list_In.
+      apply elem_of_map_to_list'.
+      apply H0.
+Qed.
+
+Lemma toggle_transaction_unsafe_preserve_trans {j wf b b' i psd tt} σ wh :
+  (get_transactions σ).1 !! wh = Some (j, wf, b, i, psd, tt) ->
+  (get_trans_gmap (get_reg_files σ, get_mail_boxes σ, get_page_tables σ, get_current_vm σ, get_mem σ,
+                   (<[wh := (j, wf, b', i, psd, tt)]> (get_transactions σ).1, (get_transactions σ).2))) = get_trans_gmap σ.
+Proof.
+  intros H.
+  rewrite /get_trans_gmap /get_transactions_gmap //=.
+  apply map_eq.
+  intros x.
+  destruct (list_to_map
+              (map (λ p : Addr * transaction, (p.1, (p.2.1.1.1.1.1, p.2.1.1.1.1.2, p.2.1.1.2, p.2.1.2, p.2.2)))
+                   (map_to_list (<[wh := (j, wf, b', i, psd, tt)]> (get_transactions σ).1))) !! x) eqn:Heqn.
+  - apply elem_of_list_to_map_2 in Heqn.
+    apply elem_of_list_In in Heqn.
+    apply in_map_iff in Heqn.
+    destruct Heqn as [y [Heqn1 Heqn2]].
+    apply elem_of_list_In in Heqn2.
+    apply elem_of_map_to_list' in Heqn2.
+    inversion Heqn1; subst; clear Heqn1.
+    symmetry.
+    apply elem_of_list_to_map_1'.
+    + intros t P.
+      apply elem_of_list_In in P.
+      apply in_map_iff in P.
+      destruct P as [r [P1 P2]].
+      apply elem_of_list_In in P2.
+      apply elem_of_map_to_list' in P2.
+      inversion P1; subst; clear P1.
+      destruct (decide (wh = y.1)).
+      * simplify_eq.
+        rewrite lookup_insert in Heqn2.
+        inversion Heqn2; subst; clear Heqn2.
+        simpl.
+        rewrite H1 in P2.
+        rewrite P2 in H.
+        inversion H; subst; clear H.
+        rewrite H3; reflexivity.
+      * rewrite H1 in P2.
+        rewrite lookup_insert_ne in Heqn2; auto.
+        rewrite P2 in Heqn2.
+        inversion Heqn2; subst; clear Heqn2; reflexivity.
+    + apply elem_of_list_In.
+      apply in_map_iff.
+      destruct (decide (wh = y.1)).
+      * simplify_eq.
+        rewrite lookup_insert in Heqn2.
+        inversion Heqn2; subst; clear Heqn2.
+        simpl.
+        exists (y.1, ((j, wf, b, i, psd, tt))).
+        split; auto.
+        apply elem_of_list_In.
+        apply elem_of_map_to_list'.
+        simpl.
+        assumption.
+      * rewrite lookup_insert_ne in Heqn2; auto.
+        exists (y.1, y.2).
+        split; auto.
+        apply elem_of_list_In.
+        apply elem_of_map_to_list'.
+        simpl.
+        assumption.
+  - destruct (decide (wh = x)).
+    + subst wh.
+      symmetry.
+      apply not_elem_of_list_to_map_1.
+      intros P.
+      apply not_elem_of_list_to_map_2 in Heqn.
+      apply Heqn.
+      rewrite <-list_fmap_compose.
+      rewrite <-list_fmap_compose in P.
+      rewrite /compose.
+      rewrite /compose in P.
+      simpl in *.
+      apply elem_of_list_In.
+      apply in_map_iff.
+      apply elem_of_list_In in P.
+      apply in_map_iff in P.
+      destruct P as [t [P1 P2]].
+      exists (t.1, (j, wf, b', i, psd, tt)).
+      split; auto.
+      apply elem_of_list_In.
+      apply elem_of_map_to_list'.
+      simpl.
+      subst x.
+      apply lookup_insert.
+    + symmetry.
+      apply not_elem_of_list_to_map_1.
+      intros P.
+      apply not_elem_of_list_to_map_2 in Heqn.
+      apply Heqn.
+      rewrite <-list_fmap_compose.
+      rewrite <-list_fmap_compose in P.
+      rewrite /compose.
+      rewrite /compose in P.
+      simpl in *.
+      apply elem_of_list_In.
+      apply in_map_iff.
+      apply elem_of_list_In in P.
+      apply in_map_iff in P.
+      destruct P as [t [P1 P2]].
+      apply elem_of_list_In in P2.
+      destruct t as [t1 t2].
+      apply elem_of_map_to_list in P2.
+      exists (t1, t2).
+      split; auto.
+      apply elem_of_list_In.
+      apply elem_of_map_to_list'.
+      simpl.
+      subst x.
+      simpl in n.
+      rewrite lookup_insert_ne; auto.
+Qed.
+
+Lemma get_retri_gmap_to_get_transaction σ wh {j wf b i psd tt}:
+  (<[wh:=b]> (get_retri_gmap σ)) =
+  (get_retri_gmap
+     (get_reg_files σ, get_mail_boxes σ, get_page_tables σ,
+      get_current_vm σ, get_mem σ,
+      (<[wh := (j, wf, b, i, psd, tt)]>
+       (get_transactions σ).1, (get_transactions σ).2))).
+Proof.
+  rewrite /get_retri_gmap.
+  rewrite /get_transactions_gmap.
+  apply map_eq.
+  intros x.
+  destruct (list_to_map
+              (map (λ p : Addr * transaction, (p.1, p.2.1.1.1.2))
+                   (map_to_list
+                      (get_transactions
+                         (get_reg_files σ, get_mail_boxes σ, get_page_tables σ,
+                          get_current_vm σ, get_mem σ,
+                          (<[wh := (j, wf, b, i, psd, tt)]> (get_transactions σ).1, (get_transactions σ).2))).1))
+              !! x) eqn:Heqn.
+  - apply elem_of_list_to_map_2 in Heqn.
+    apply elem_of_list_In in Heqn.
+    apply in_map_iff in Heqn.
+    destruct Heqn as [y [Heqn1 Heqn2]].
+    apply elem_of_list_In in Heqn2.
+    apply elem_of_map_to_list' in Heqn2.
+    inversion Heqn1; subst; clear Heqn1.
+    destruct (decide (wh = y.1)).
+    + subst.
+      rewrite /get_transactions in Heqn2.
+      simpl in Heqn2.
+      apply lookup_insert_rev in Heqn2.
+      inversion Heqn2; subst; clear Heqn2.
+      simpl.
+      apply lookup_insert.
+    + rewrite /get_transactions in Heqn2.
+      simpl in Heqn2.
+      rewrite ->lookup_insert_Some in Heqn2.
+      destruct Heqn2 as [H | H].
+      destruct H; done.
+      destruct H as [_ H].
+      rewrite ->lookup_insert_Some.
+      right.
+      split; auto.
+      apply elem_of_list_to_map_1'.
+      intros y' Q.
+      apply elem_of_list_In in Q.
+      apply in_map_iff in Q.
+      destruct Q as [r [Q1 Q2]].
+      inversion Q1; subst; clear Q1.
+      rewrite (surjective_pairing r) in Q2.
+      apply elem_of_list_In in Q2.
+      apply elem_of_map_to_list' in Q2.
+      simpl in Q2.
+      rewrite /get_transactions in Q2.
+      rewrite H1 in Q2.
+      rewrite Q2 in H.
+      inversion H; subst; clear H.
+      f_equal.
+      apply elem_of_list_In.
+      apply in_map_iff.
+      exists (y.1, y.2).
+      split; auto.
+      rewrite /get_transactions.
+      apply elem_of_list_In.
+      apply elem_of_map_to_list.
+      assumption.
+  - rewrite <-not_elem_of_list_to_map in Heqn.
+    simpl in Heqn.
+    destruct (decide (wh = x)).
+    + subst.
+      exfalso.
+      apply Heqn.
+      rewrite <-list_fmap_compose.
+      rewrite /compose.
+      simpl.
+      apply elem_of_list_In.
+      apply in_map_iff.
+      exists (x, (j, wf, b, i, psd, tt)).
+      split; auto.
+      apply elem_of_list_In.
+      apply elem_of_map_to_list'.
+      simpl.
+      rewrite lookup_insert; auto.
+    + rewrite lookup_insert_ne; auto.
+      rewrite <-not_elem_of_list_to_map.
+      intros H.
+      apply Heqn.
+      rewrite ->elem_of_list_In in H.
+      apply in_map_iff in H.
+      destruct H as [x' [H1 H2]]; subst.
+      apply in_map_iff in H2.
+      destruct H2 as [x'' [H2 H3]].
+      inversion H2; subst.
+      rewrite elem_of_list_In.
+      apply in_map_iff.
+      exists (x''.1, x''.2.1.1.1.2).
+      split; auto.
+      apply in_map_iff.
+      exists (x''.1, x''.2).
+      split; auto.
+      rewrite <-elem_of_list_In.
+      apply elem_of_map_to_list'.
+      simpl.
+      rewrite lookup_insert_ne; auto.
+      rewrite <-elem_of_map_to_list.
+      rewrite elem_of_list_In.
+      rewrite <-surjective_pairing.
+      assumption.
+Qed.
+
+Lemma insert_transaction_update_trans σ h tran:
+  (get_trans_gmap (insert_transaction σ h tran))
+  = <[h:= (tran.1.1.1.1.1,tran.1.1.1.1.2,tran.1.1.2,tran.1.2, tran.2)]>(get_trans_gmap σ).
+Proof.
+  apply (insert_transaction_update_transactions
+           (λ tran, (tran.1.1.1.1.1,tran.1.1.1.1.2,tran.1.1.2,tran.1.2, tran.2))).
+Qed.
+
+Lemma insert_transaction_update_hpool σ h tran:
+  (get_hpool_gset (insert_transaction σ h tran)) = ((get_hpool_gset σ) ∖ {[h]}).
+Proof. rewrite /insert_transaction /get_hpool_gset /= //. Qed.
+
+Lemma insert_transaction_update_retri σ h tran:
+  (get_retri_gmap (insert_transaction σ h tran)) = <[h:=tran.1.1.1.2]>(get_retri_gmap σ).
+Proof.
+  apply (insert_transaction_update_transactions (λ tran, tran.1.1.1.2)).
+Qed.
+
+
+  Lemma get_transactions_gmap_preserve_dom {Info:Type} {σ} (proj : transaction->Info):
+   dom (gset handle) (get_transactions_gmap σ proj) = dom (gset handle) (get_transactions σ).1.
+  Proof.
+   apply set_eq.
+   split.
+   - intros.
+     apply elem_of_dom.
+     apply elem_of_dom in H.
+     destruct H.
+     rewrite /get_trans_gmap in H.
+     apply  elem_of_list_to_map_2 in H.
+     inv_map_in.
+     apply elem_of_list_In in H0.
+     destruct x1.
+     apply (elem_of_map_to_list) in H0.
+     inversion H;subst f.
+     eexists.
+     done.
+   - intros.
+     apply elem_of_dom.
+     apply elem_of_dom in H.
+     destruct H.
+     rewrite /get_trans_gmap.
+     exists (proj x0).
+     apply elem_of_list_to_map'.
+     intros.
+     inv_map_in.
+     inversion H1;subst x.
+     clear H5 H1.
+     apply elem_of_list_In in H2.
+     destruct x1.
+     apply (elem_of_map_to_list) in H2.
+     simpl in *.
+     rewrite H2 in H.
+     inversion H;subst t.
+     done.
+     inv_map_in.
+     exists (x,x0).
+     split;[done|].
+     apply elem_of_list_In.
+     by apply (elem_of_map_to_list).
+  Qed.
+
+  Lemma get_trans_gmap_preserve_dom {σ}:
+   dom (gset handle) (get_trans_gmap σ) = dom (gset handle) (get_transactions σ).1.
+  Proof.
+    apply get_transactions_gmap_preserve_dom.
+  Qed.
+
+  Lemma get_retri_gmap_preserve_dom {σ}:
+   dom (gset handle) (get_retri_gmap σ) = dom (gset handle) (get_transactions σ).1.
+  Proof.
+    apply get_transactions_gmap_preserve_dom.
+  Qed.
