theories/rules/cmp.v
@@ -1,8 +1,7 @@
-From machine_program_logic.program_logic Require Import machine weakestpre.
-From HypVeri Require Import RAs rule_misc lifting rules.rules_base.
-From iris.proofmode Require Import tactics.
-Require Import iris.base_logic.lib.ghost_map.
-Require Import stdpp.fin.
+From machine_program_logic.program_logic Require Import weakestpre.
+From HypVeri Require Import lifting rules.rules_base.
+From HypVeri.algebra Require Import base mem reg pagetable.
+From HypVeri.lang Require Import lang_extra reg_extra.
 
 Section cmp.
 
@@ -30,11 +29,11 @@ Proof.
   subst src dst.
   inversion Hvalidra as [ HneqPCa HneqNZa ].
   (* valid regs *)
-  iDestruct ((gen_reg_valid3 σ1 i PC ai ra w3 NZ w4 Hcur HneqPCa) with "Hreg Hpc Hra Hnz") as "[%HPC [%Hra %HNZ]]";eauto.
+  iDestruct ((gen_reg_valid3 i PC ai ra w3 NZ w4 Hcur HneqPCa) with "Hreg Hpc Hra Hnz") as "[%HPC [%Hra %HNZ]]";eauto.
   (* valid pt *)
   iDestruct ((gen_access_valid_addr ai pi) with "Haccess Hacc") as %Hacc;eauto.
   (* valid mem *)
-  iDestruct (gen_mem_valid σ1 ai w1  with "Hmem Hapc") as %Hmem.
+  iDestruct (gen_mem_valid ai w1  with "Hmem Hapc") as %Hmem.
   iSplit.
   - (* reducible *)
     iPureIntro.
@@ -102,11 +101,11 @@ Proof.
   destruct  Hvalidra as [ HneqPCa HneqNZa ].
   destruct  Hvalidrb as [ HneqPCb HneqNZb ].
   (* valid regs *)
-  iDestruct ((gen_reg_valid4 σ1 i PC ai ra w2 rb w3 NZ w4 Hcur) with "Hreg Hpc Hra Hrb Hnz") as "[%HPC [%Hra [%Hrb %HNZ]]]";eauto.
+  iDestruct ((gen_reg_valid4 i PC ai ra w2 rb w3 NZ w4 Hcur) with "Hreg Hpc Hra Hrb Hnz") as "[%HPC [%Hra [%Hrb %HNZ]]]";eauto.
   (* valid pt *)
   iDestruct ((gen_access_valid_addr ai pi) with "Haccess Hacc") as %Hacc;eauto.
   (* valid mem *)
-  iDestruct (gen_mem_valid σ1 ai w1  with "Hmem Hapc") as %Hmem.
+  iDestruct (gen_mem_valid ai w1  with "Hmem Hapc") as %Hmem.
   iSplit.
   - (* reducible *)
     iPureIntro.
