theories/rules/donate.v
@@ -1,8 +1,8 @@
 From machine_program_logic.program_logic Require Import weakestpre.
 From iris.algebra Require Import gset.
-From HypVeri Require Import transaction rule_misc lifting rules.rules_base.
+From HypVeri Require Import lifting rules.rules_base.
 From HypVeri.algebra Require Import base mem reg pagetable mailbox trans.
-Require Import stdpp.fin.
+From HypVeri.lang Require Import lang_extra reg_extra mem_extra pagetable_extra trans_extra.
 
 Section donate.
 
